bin/output/main_int_0.dfy
@@ -2,37 +2,30 @@
 include "utils.dfy"
 
 /******************************* UDTS ***************************************/
-class Average{
+class Sum{
 }
 
 
 /***************************** DO MAP ***************************************/
 
-function emit0(data: seq<int>, i0: int, i: int, loop0: bool) : seq<(int, int)>
+function emit0(data: seq<int>, i0: int, i: int, loop0: bool) : seq<(int, (int,int))>
 	requires 0 <= i < |data|
-	ensures emit0(data, i0, i, loop0) == [(2,(data[i]+19)+(data[i]+2))]
+	ensures emit0(data, i0, i, loop0) == [(1,(data[i]+data[i],data[i]))]
 {
-	[(2,(data[i]+19)+(data[i]+2))]
-}
-
-function emit1(data: seq<int>, i0: int, i: int, loop0: bool) : seq<(int, int)>
-	requires 0 <= i < |data|
-	ensures emit1(data, i0, i, loop0) == [(1,data[i])]
-{
-	[(1,data[i])]
+	[(1,(data[i]+data[i],data[i]))]
 }
 
 
-function domap (data: seq<int>, i0: int, i: int, loop0: bool) : seq<(int, int)>
+function domap (data: seq<int>, i0: int, i: int, loop0: bool) : seq<(int, (int,int))>
     requires 0 <= i < |data|
-    ensures domap(data, i0, i, loop0) == emit0(data, i0, i, loop0) + emit1(data, i0, i, loop0)
+    ensures domap(data, i0, i, loop0) == emit0(data, i0, i, loop0)
 {
-    emit0(data, i0, i, loop0) + emit1(data, i0, i, loop0)
+    emit0(data, i0, i, loop0)
 }
 
 /***************************** MAPPER ***************************************/
 
-function mapper (data: seq<int>, i0: int, i: int, loop0: bool) : seq<(int, int)>
+function mapper (data: seq<int>, i0: int, i: int, loop0: bool) : seq<(int, (int,int))>
     requires 0 <= i <= |data|
 {
     if i == 0 then []
@@ -41,83 +34,53 @@ function mapper (data: seq<int>, i0: int, i: int, loop0: bool) : seq<(int, int)>
 
 /***************************** DO REDUCE ************************************/
 
-function doreduce(input: seq<(int, int)>, key: int, loop0: bool) : int
+function doreduce(input: seq<(int, (int,int))>, key: int, loop0: bool) : int
     ensures (|input| > 0 && input[0].0 == key) ==> 
-        doreduce(input, key, loop0) == (if key == 1 then ((doreduce(input[1..], key, loop0)+input[0].1)) else if key == 2 then ((doreduce(input[1..], key, loop0)+1)) else ((doreduce(input[1..], key, loop0)+1)))
+        doreduce(input, key, loop0) == (if key == 1 then ((input[0].1.1+doreduce(input[1..], key, loop0))) else ((input[0].1.1+doreduce(input[1..], key, loop0))))
     ensures (|input| > 0 && input[0].0 != key) ==> 
         doreduce(input, key, loop0) == doreduce(input[1..], key, loop0)
 {
-    if input == [] then (if key == 1 then 0 else if key == 2 then 0 else 0 )
-    else if input[0].0 == key then (if key == 1 then ((doreduce(input[1..], key, loop0)+input[0].1)) else if key == 2 then ((doreduce(input[1..], key, loop0)+1)) else ((doreduce(input[1..], key, loop0)+1)))
+    if input == [] then (if key == 1 then 0 else 0 )
+    else if input[0].0 == key then (if key == 1 then ((input[0].1.1+doreduce(input[1..], key, loop0))) else ((input[0].1.1+doreduce(input[1..], key, loop0))))
     else doreduce(input[1..], key, loop0)
 }
 
 /******************************* HARNESS ************************************/    
 
-lemma LemmaCSG_sum (a: seq<(int, int)>, b: seq<(int, int)>, key: int, loop0: bool)
-	requires key == 1
-ensures doreduce(a+b, key, loop0) == ((doreduce(a, key, loop0)+doreduce(b, key, loop0)))
-{
-	if a != []
-	{
-		LemmaCSG_sum(a[1..], b, key, loop0);
-		assert a + b == [a[0]] + (a[1..] + b);
-	}
-}
-
-lemma LemmaCSG_count (a: seq<(int, int)>, b: seq<(int, int)>, key: int, loop0: bool)
-	requires key == 2
-ensures doreduce(a+b, key, loop0) == ((doreduce(a, key, loop0)+1))
-{
-	if a != []
-	{
-		LemmaCSG_count(a[1..], b, key, loop0);
-		assert a + b == [a[0]] + (a[1..] + b);
-	}
-}
-
-
-
-
-predicate loopInvariant (data: seq<int>, count: int, count0: int, sum: int, sum0: int, i: int, i0: int, loop0: bool)
+predicate loopInvariant (data: seq<int>, sum: int, sum0: int, i: int, i0: int, loop0: bool)
     
 {
     0 <= i <= |data| &&
-	(sum == (doreduce(mapper(data,i0,i,loop0),1, loop0))) &&
-	(count == (doreduce(mapper(data,i0,i,loop0),2, loop0)))
+	(sum == (doreduce(mapper(data,i0,i,loop0),1, loop0)))
 }
 
-predicate postCondition (data: seq<int>, count: int, count0: int, sum: int, sum0: int, i: int, i0: int, loop0: bool)
+predicate postCondition (data: seq<int>, sum: int, sum0: int, i: int, i0: int, loop0: bool)
     
 {
     i == |data| &&
-	(sum == (doreduce(mapper(data,i0,i,loop0),1, loop0))) &&
-	(count == (doreduce(mapper(data,i0,i,loop0),2, loop0)))
+	(sum == (doreduce(mapper(data,i0,i,loop0),1, loop0)))
 }
 
-method harness (data: seq<int>, sum: int, count: int, i: int)
+method harness (data: seq<int>, sum: int, i: int)
     
 {
     var sum0 := 0;
-	var count0 := 0;
 	var loop0 := false;
 	var i0 := 0;
 	
-    assert loopInvariant(data,0,0,0,0,0,0,loop0);
+    assert loopInvariant(data,0,0,0,0,loop0);
 
-	if(loopInvariant(data,count,0,sum,0,i,0,loop0) && (i<|data|))
+	if(loopInvariant(data,sum,0,i,0,loop0) && (i<|data|))
 	{
-		var ind_count := count;
-		ind_count := (count+1);
 		var ind_sum := sum;
 		ind_sum := (sum+data[i]);
 		var ind_i := i;
 		ind_i := (i+1);
-		assert loopInvariant(data,ind_count,0,ind_sum,0,ind_i,0,loop0);
+		assert loopInvariant(data,ind_sum,0,ind_i,0,loop0);
 	}
 
-	if(loopInvariant(data,count,0,sum,0,i,0,loop0) && !(i<|data|))
+	if(loopInvariant(data,sum,0,i,0,loop0) && !(i<|data|))
 	{
-		assert postCondition(data,count,0,sum,0,i,0,loop0);
+		assert postCondition(data,sum,0,i,0,loop0);
 	}
 }
