bin/output/main_int_0_CSG.dfy
@@ -1,0 +1,24 @@
+function doreduce(input: seq<(int, (int,int))>, key: int, loop0: bool) : int
+    ensures (|input| > 0 && input[0].0 == key) ==> 
+        doreduce(input, key, loop0) == (if key == 1 then ((input[0].1.1+doreduce(input[1..], key, loop0))) else ((input[0].1.1+doreduce(input[1..], key, loop0))))
+    ensures (|input| > 0 && input[0].0 != key) ==> 
+        doreduce(input, key, loop0) == doreduce(input[1..], key, loop0)
+{
+    if input == [] then (if key == 1 then 0 else 0 )
+    else if input[0].0 == key then (if key == 1 then ((input[0].1.1+doreduce(input[1..], key, loop0))) else ((input[0].1.1+doreduce(input[1..], key, loop0))))
+    else doreduce(input[1..], key, loop0)
+}
+
+/******************************* HARNESS ************************************/    
+
+lemma LemmaCSG_sum (a: seq<(int, (int,int))>, b: seq<(int, (int,int))>, key: int, loop0: bool)
+	requires key == 1
+ensures doreduce(a+b, key, loop0) == (doreduce(a, key, loop0) + doreduce(b, key, loop0))
+{
+	if a != []
+	{
+		LemmaCSG_sum(a[1..], b, key, loop0);
+		assert a + b == [a[0]] + (a[1..] + b);
+	}
+}
+
