bin/templates/dafny_skeleton2.dfy
@@ -1,0 +1,14 @@
+function doreduce(input: <domap-emit-type>, key: <doreduce-key-type><reducer-args-decl>) : <output-type>
+    ensures (|input| > 0 && input[0].0 == key) ==> 
+        doreduce(input, key<reducer-args-call>) == (<reduce-exp>)
+    ensures (|input| > 0 && input[0].0 != key) ==> 
+        doreduce(input, key<reducer-args-call>) == doreduce(input[1..], key<reducer-args-call>)
+{
+    if input == [] then (<reduce-init-value> )
+    else if input[0].0 == key then (<reduce-exp>)
+    else doreduce(input[1..], key<reducer-args-call>)
+}
+
+/******************************* HARNESS ************************************/    
+
+<reduce-exp-lemma>
